chore: fill in full strategy

Fp/Theorems/PackedUnpackedRel/Basic.lean
@@ -4,13 +4,13 @@ import Fp.Theorems.UnpackedFloat.ToRat
 import Fp.EUnpackedFloat.Basic
 import Fp.Basic
 
+
 /--
 An unpacked float is related to a packed float
 iff they have the same rational value and the same sign.
 -/
-def UnpackedFloat.Rel (uf : UnpackedFloat ef uf)
-(pf : PackedFloat ep sp) :=
-  uf.toRat' = pf.toRat ∧ uf.sign = pf.sign
+def UnpackedFloat.Rel (uf : UnpackedFloat e s) (pf : PackedFloat ep sp) :=
+  uf.toRat' = pf.toRat ∧ uf.sign = pf.sign -- ∧ ¬ pf.isInfinite ∧ ¬ pf.isNaN
 
 @[grind =>]
 theorem UnpackedFloat.Rel_of_toRat_eq_toRat_and_sign (uf : UnpackedFloat ef uf) (pf : PackedFloat ep sp)
